deps/poulet4/lib/Typed.v
@@ -41,10 +41,10 @@ Section Typed.
   | TypBool
   | TypString
   | TypInteger
-  | TypInt (width: nat)
-  | TypBit (width: nat)
-  | TypVarBit (width: nat)
-  | TypArray (typ: P4Type) (size: nat)
+  | TypInt (width: N)
+  | TypBit (width: N)
+  | TypVarBit (width: N)
+  | TypArray (typ: P4Type) (size: N)
   | TypTuple (types: list P4Type)
   | TypList (types: list P4Type)
   | TypRecord (fields: P4String.AList tags_t P4Type)
@@ -75,7 +75,7 @@ Section Typed.
   | MkFunctionType (type_params: list P4String) (parameters: list P4Parameter)
                    (kind: FunctionKind) (ret: P4Type)
   with P4Parameter :=
-  | MkParameter (opt: bool) (direction: direction) (typ: P4Type) (default_arg_id: option nat) (variable: P4String).
+  | MkParameter (opt: bool) (direction: direction) (typ: P4Type) (default_arg_id: option N) (variable: P4String).
 
   Inductive StmType :=
   | StmUnit
