deps/poulet4/lib/Typing.v
@@ -1,0 +1,728 @@
+Require Import Poulet4.Semantics Poulet4.Typed
+        Poulet4.Syntax Coq.NArith.BinNat Coq.Lists.List
+        Poulet4.Value Coq.micromega.Lia Poulet4.Utils.
+Import ListNotations.
+Require Poulet4.P4String.
+
+Section ValueTyping.
+  Context {tags_t : Type}.
+
+  Notation typ := (@P4Type tags_t).
+
+  Section Val.
+    Context {A : Type}.
+    Notation V := (@ValueBase tags_t A).
+    Notation senum_env := (@IdentMap.t tags_t (P4String.AList tags_t V)).
+    
+    (* TODO:
+       What constraints do we need on:
+       - fixed-width numeric types?
+       - headers (unions & stacks)?
+       - senum values: see comments below.
+       - needs to be parameterized by bit type. *)
+
+    Variable (gsenum : senum_env).
+
+    Inductive val_typ : V -> typ -> Prop :=
+    | typ_null :
+        val_typ ValBaseNull TypVoid
+    | typ_bool : forall b,
+        val_typ (ValBaseBool b) TypBool
+    | typ_integer : forall v,
+        val_typ (ValBaseInteger v) TypInteger
+    | typ_bit : forall v,
+        val_typ (ValBaseBit v) (TypBit (N.of_nat (length v)))
+    | typ_int : forall v,
+        val_typ (ValBaseInt v) (TypInt (N.of_nat (length v)))
+    | typ_varbit : forall n v,
+        N.to_nat n < length v ->
+        val_typ (ValBaseVarbit n v) (TypVarBit n)
+    | typ_string : forall s,
+        val_typ (ValBaseString s) TypString
+    | typ_tuple : forall vs ts,
+        Forall2 val_typ vs ts ->
+        val_typ (ValBaseTuple vs) (TypTuple ts)
+    | typ_record : forall vs ts,
+        AList.all_values val_typ vs ts ->
+        val_typ (ValBaseRecord vs) (TypRecord ts)
+    | typ_error : forall err,
+        val_typ (ValBaseError err) TypError
+    | typ_matchkind : forall mk,
+        val_typ (ValBaseMatchKind mk) TypMatchKind
+    | typ_struct : forall vs ts,
+        AList.all_values val_typ vs ts ->
+        val_typ (ValBaseStruct vs) (TypStruct ts)
+    | typ_header : forall b vs ts,
+        AList.all_values val_typ vs ts ->
+        val_typ (ValBaseHeader vs b) (TypHeader ts)
+    | typ_union : forall vs ts,
+        AList.all_values val_typ vs ts ->
+        val_typ (ValBaseUnion vs) (TypHeaderUnion ts)
+    | typ_stack : forall s n vs ts,
+        length vs = N.to_nat s ->
+        Forall (fun v => val_typ v (TypHeader ts)) vs ->
+        val_typ (ValBaseStack vs s n) (TypArray (TypHeader ts) n)
+    | typ_enumfield : forall ename member members,
+        In member members ->
+        val_typ
+          (ValBaseEnumField ename member)
+          (TypEnum ename None members)
+    | typ_senumfield : forall ename member v t fields,
+        IdentMap.get ename gsenum = Some fields ->
+        AList.get fields member = Some v ->
+        val_typ v t ->
+        val_typ
+          (ValBaseSenumField ename member v)
+          (TypEnum ename (Some t) (List.map fst fields))
+    (* TODO: what is a [ValBaseSenum _], and what is its type?
+       It seems to be something in [gsenum],
+       but should it be a value? *)
+    (*| typ_senum : forall fields ename t,
+        IdentMap.get ename gsenum = Some fields ->
+        Forall (fun xv => val_typ gsenum (snd xv) t) fields ->
+        val_typ
+          gsenum (ValBaseSenum fields)
+          (TypEnum ename (Some t) (List.map fst fields))*).
+
+    Section ValTypInd.
+      Variable P : V -> typ -> Prop.
+
+      Hypothesis HNull : P ValBaseNull TypVoid.
+      Hypothesis HBool : forall b, P (ValBaseBool b) TypBool.
+      Hypothesis HInteger : forall z, P (ValBaseInteger z) TypInteger.
+      Hypothesis HBit : forall bits,
+          P (ValBaseBit bits) (TypBit (N.of_nat (length bits))).
+      Hypothesis HInt : forall bits,
+          P (ValBaseInt bits) (TypInt (N.of_nat (length bits))).
+      Hypothesis HVarbit : forall n bits,
+          N.to_nat n < length bits ->
+          P (ValBaseVarbit n bits) (TypVarBit n).
+      Hypothesis HString : forall s,
+          P (ValBaseString s) TypString.
+      Hypothesis HTuple : forall vs ts,
+          Forall2 val_typ vs ts ->
+          Forall2 P vs ts ->
+          P (ValBaseTuple vs) (TypTuple ts).
+      Hypothesis HRecord : forall vs ts,
+          AList.all_values val_typ vs ts ->
+          AList.all_values P vs ts ->
+          P (ValBaseRecord vs) (TypRecord ts).
+      Hypothesis HError : forall err,
+          P (ValBaseError err) TypError.
+      Hypothesis HMatchkind : forall mk,
+          P (ValBaseMatchKind mk) TypMatchKind.
+      Hypothesis HStruct : forall vs ts,
+          AList.all_values val_typ vs ts ->
+          AList.all_values P vs ts ->
+          P (ValBaseStruct vs) (TypStruct ts).
+      Hypothesis HHeader : forall b vs ts,
+          AList.all_values val_typ vs ts ->
+          AList.all_values P vs ts ->
+          P (ValBaseHeader vs b) (TypHeader ts).
+      Hypothesis HUnion : forall vs ts,
+          AList.all_values val_typ vs ts ->
+          AList.all_values P vs ts ->
+          P (ValBaseUnion vs) (TypHeaderUnion ts).
+      Hypothesis HStack : forall s n vs ts,
+          length vs = N.to_nat s ->
+          Forall (fun v => val_typ v (TypHeader ts)) vs ->
+          Forall (fun v => P v (TypHeader ts)) vs ->
+          P (ValBaseStack vs s n) (TypArray (TypHeader ts) n).
+      Hypothesis HEnum : forall ename member members,
+          In member members ->
+          P
+            (ValBaseEnumField ename member)
+            (TypEnum ename None members).
+      Hypothesis HSenum : forall ename member v t fields,
+          IdentMap.get ename gsenum = Some fields ->
+          AList.get fields member = Some v ->
+          val_typ v t ->
+          P v t ->
+          P
+            (ValBaseSenumField ename member v)
+            (TypEnum ename (Some t) (List.map fst fields)).
+
+      Definition custom_val_typ_ind :
+        forall (v : V) (t : typ), val_typ v t -> P v t :=
+        fix vtind (v : V) (t : typ) (H : val_typ v t) : P v t :=
+          let fix lind {vs : list V} {ts : list typ}
+                  (H : Forall2 val_typ vs ts)
+              : Forall2 P vs ts :=
+              match H with
+              | Forall2_nil _ => Forall2_nil _
+              | Forall2_cons _ _ Hh Ht =>
+                Forall2_cons _ _ (vtind _ _ Hh) (lind Ht)
+              end in
+          let fix alind
+                  {vs : AList.AList (P4String.t _) V _}
+                  {ts : AList.AList (P4String.t _) typ _}
+                  (H : AList.all_values val_typ vs ts)
+              : AList.all_values P vs ts :=
+              match H with
+              | Forall2_nil _ => Forall2_nil _
+              | Forall2_cons _ _ (conj Hx Hh) Ht =>
+                Forall2_cons _ _ (conj Hx (vtind _ _ Hh)) (alind Ht)
+              end in
+          let fix same_typ_ind {vs : list V} {t : typ}
+                  (H : Forall (fun v => val_typ v t) vs)
+              : Forall (fun v => P v t) vs :=
+              match H with
+              | Forall_nil _ => Forall_nil _
+              | Forall_cons _ Hh Ht =>
+                Forall_cons _ (vtind _ _ Hh) (same_typ_ind Ht)
+              end in
+          match H with
+          | typ_null => HNull
+          | typ_bool b => HBool b
+          | typ_integer z => HInteger z
+          | typ_bit bits => HBit bits
+          | typ_int bits => HInt bits
+          | typ_varbit _ _ H => HVarbit _ _ H
+          | typ_string s => HString s
+          | typ_tuple _ _ H => HTuple _ _ H (lind H)
+          | typ_record _ _ H => HRecord _ _ H (alind H)
+          | typ_error err => HError err
+          | typ_matchkind mk => HMatchkind mk
+          | typ_struct _ _ H => HStruct _ _ H (alind H)
+          | typ_header b _ _ H => HHeader b _ _ H (alind H)
+          | typ_union _ _ H => HUnion _ _ H (alind H)
+          | typ_stack _ n _ _ Hl H => HStack _ n _ _ Hl H (same_typ_ind H)
+          | typ_enumfield x _ _ H => HEnum x _ _ H
+          | typ_senumfield _ _ _ _ _ H1 H2 Hv =>
+            HSenum _ _ _ _ _ H1 H2 Hv (vtind _ _ Hv)
+          end.
+    End ValTypInd.
+  End Val.
+
+  Section RelTyp.
+    Context {A B : Type}.
+    Notation VA := (@ValueBase tags_t A).
+    Notation VB := (@ValueBase tags_t B).
+
+    Local Hint Constructors val_typ : core.
+    
+    Section Map.
+      Variable (f : A -> B).
+      
+      Lemma ValueBaseMap_preserves_type : forall gs v t,
+          val_typ gs v t ->
+          val_typ
+            (FuncAsMap.map_map (AList.map_values (ValueBaseMap f)) gs)
+            (ValueBaseMap f v) t.
+      Proof.
+        intros gs v t Hv;
+          induction Hv using @custom_val_typ_ind;
+          simpl in *; auto.
+        - replace (length bits)
+            with (length (map f bits))
+            by (rewrite map_length; reflexivity); auto.
+        - replace (length bits)
+            with (length (map f bits))
+            by (rewrite map_length; reflexivity); auto.
+        - constructor; rewrite map_length; auto.
+        - rewrite Forall2_map_l in H0; auto.
+        - constructor.
+          unfold AList.all_values in *.
+          rewrite Forall2_conj in *;
+            destruct H0 as [Hnames Hvts]; split.
+          + clear Hvts.
+            rewrite Forall2_map_both in *.
+            rewrite map_fst_map, map_id.
+            assumption.
+          + clear Hnames.
+            rewrite Forall2_map_both, map_snd_map,
+            map_map, <- Forall2_map_both.
+            assumption.
+        - constructor.
+          unfold AList.all_values in *.
+          rewrite Forall2_conj in *;
+            destruct H0 as [Hnames Hvts]; split.
+          + clear Hvts.
+            rewrite Forall2_map_both in *.
+            rewrite map_fst_map, map_id.
+            assumption.
+          + clear Hnames.
+            rewrite Forall2_map_both, map_snd_map,
+            map_map, <- Forall2_map_both.
+            assumption.
+        - constructor.
+          unfold AList.all_values in *.
+          rewrite Forall2_conj in *;
+            destruct H0 as [Hnames Hvts]; split.
+          + clear Hvts.
+            rewrite Forall2_map_both in *.
+            rewrite map_fst_map, map_id.
+            assumption.
+          + clear Hnames.
+            rewrite Forall2_map_both, map_snd_map,
+            map_map, <- Forall2_map_both.
+            assumption.
+        - constructor.
+          unfold AList.all_values in *.
+          rewrite Forall2_conj in *;
+            destruct H0 as [Hnames Hvts]; split.
+          + clear Hvts.
+            rewrite Forall2_map_both in *.
+            rewrite map_fst_map, map_id.
+            assumption.
+          + clear Hnames.
+            rewrite Forall2_map_both, map_snd_map,
+            map_map, <- Forall2_map_both.
+            assumption.
+        - constructor.
+          + rewrite map_length; assumption.
+          + rewrite Forall_map.
+            unfold Basics.compose.
+            assumption.
+        - replace (map fst fields) with
+              (map fst (AList.map_values (ValueBaseMap f) fields)).
+          constructor; auto.
+          + unfold IdentMap.get,
+            FuncAsMap.get, FuncAsMap.map_map in *.
+            rewrite H; reflexivity.
+          + rewrite AList.get_map_values, H0; reflexivity.
+          + unfold AList.map_values.
+            rewrite map_fst_map, map_id; reflexivity.
+      Qed.
+    End Map.
+
+    Section Rel.
+      Variable (R : A -> B -> Prop).
+      
+      Lemma exec_val_preserves_typ : forall va vb,
+          exec_val R va vb ->
+          forall gsa gsb t,
+            FuncAsMap.related
+              (AList.all_values (exec_val R))
+              gsa gsb ->
+            val_typ gsa va t -> val_typ gsb vb t.
+      Proof.
+        (* TODO: need induction principle for [exec_val]. *)
+      Admitted.
+    End Rel.
+  End RelTyp.
+End ValueTyping.
+    
+Section TypingDefs.
+  Context {tags_t : Type} {dummy : Inhabitant tags_t}.
+
+  Notation typ := (@P4Type tags_t).
+  Notation expr := (@Expression tags_t).
+  Notation stmt := (@Statement tags_t).
+  Notation signal := (@signal tags_t).
+  Notation ident := (P4String.t tags_t).
+  Notation path := (list ident).
+  Notation Sval := (@ValueBase tags_t (option bool)).
+
+  (** Typing context. *)
+  Definition gamma : Type := @PathMap.t tags_t typ.
+
+  (** TODO: is this correct? *)
+  Definition typ_of_loc (l : Locator) (g : gamma) : option typ :=
+    match l with
+    | LInstance p => PathMap.get p g
+    | LGlobal   p => PathMap.get p g
+    end.
+
+  Context `{T : @Target tags_t expr}.
+
+  Notation run_expr := (@exec_expr tags_t dummy T).
+  Notation run_stmt := (@exec_stmt tags_t dummy T).
+
+  Definition envs_same (g : gamma) (st : state) : Prop :=
+    forall p : path, PathMap.get p g = None <-> PathMap.get p (fst st) = None.
+
+  Lemma envs_same_some_l : forall g st p t,
+      envs_same g st -> PathMap.get p g = Some t ->
+      exists v, PathMap.get p (fst st) = Some v.
+  Proof.
+    intros g st p t H Hgt; unfold envs_same in H.
+    destruct (PathMap.get p (fst st)) as [v |] eqn:Heq; eauto.
+    rewrite <- H, Hgt in Heq; discriminate.
+  Qed.
+
+  Lemma envs_same_some_r : forall g st p v,
+      envs_same g st -> PathMap.get p (fst st) = Some v ->
+      exists t, PathMap.get p g = Some t.
+  Proof.
+    intros g st p v H Hgt; unfold envs_same in H.
+    destruct (PathMap.get p g) as [? |] eqn:Heq; eauto.
+    rewrite H,Hgt in Heq; discriminate.
+  Qed.
+  
+  Definition envs_type (gsenum : genv_senum) (g : gamma) (st : state) : Prop :=
+    forall (p : path) (t : typ) (v : Sval),
+      PathMap.get p g = Some t ->
+      PathMap.get p (fst st) = Some v -> val_typ gsenum v t.
+
+  Definition typ_of_expr (e : expr) : typ :=
+    match e with
+    | MkExpression _ _ t _ => t
+    end.
+  (**[]*)
+  
+  (** Expression typing. *)
+  Definition expr_types (g : gamma) (e : expr) : Prop :=
+    forall (read_one_bit : option bool -> bool -> Prop)
+      (ge : genv) (p : path) (st : state),
+      envs_same g st -> envs_type ge g st ->
+      (exists v, run_expr ge read_one_bit p st e v) /\
+      forall v, run_expr ge read_one_bit p st e v ->
+           val_typ (ge_senum ge) v (typ_of_expr e).
+  (**[]*)
+
+  (** Statement typing. *)
+  Definition stmt_types (g g' : gamma) (s : stmt) : Prop :=
+    forall (read_one_bit : option bool -> bool -> Prop)
+      (ge : genv) (p : path) (st : state),
+      envs_same g st -> envs_type ge g st ->
+      (exists st' sig, run_stmt ge read_one_bit p st s st' sig) /\
+      forall st' sig, run_stmt ge read_one_bit p st s st' sig ->
+                 envs_same g' st' /\ envs_type ge g' st'.
+End TypingDefs.
+
+Notation "Γ '⊢e' e"
+  := (expr_types Γ e) (at level 80, no associativity) : type_scope.
+Notation "Γ1 '⊢s' s ⊣ Γ2"
+  := (stmt_types Γ1 Γ2 s) (at level 80, no associativity) : type_scope.
+
+(* TODO. *)
+Section Soundness.
+  Context {tags_t : Type} {dummy : Inhabitant tags_t}.
+
+  Notation typ := (@P4Type tags_t).
+  Notation expr := (@Expression tags_t).
+  Notation stmt := (@Statement tags_t).
+  Notation signal := (@signal tags_t).
+  Notation ident := (P4String.t tags_t).
+  Notation path := (list ident).
+  Notation Sval := (@ValueBase tags_t (option bool)).
+
+  Context `{T : @Target tags_t expr}.
+
+  Notation run_expr := (@exec_expr tags_t dummy T).
+  Notation run_stmt := (@exec_stmt tags_t dummy T).
+
+  Variable (Γ : @gamma tags_t).
+
+  Local Hint Unfold expr_types : core.
+  Local Hint Constructors exec_expr : core.
+  Local Hint Constructors val_typ : core.
+  
+  Ltac soundtac :=
+    autounfold with *;
+    intros rob ge p st Henvs Henvt;
+    split; eauto;
+    try (intros v Hrn; inversion Hrn; subst; cbn; eauto).
+  
+  Lemma bool_sound : forall tag b dir,
+      Γ ⊢e MkExpression tag (ExpBool b) TypBool dir.
+  Proof.
+    intros; soundtac.
+  Qed.
+  
+  Lemma arbitrary_int_sound : forall tag i z dir,
+      Γ ⊢e
+        MkExpression
+        tag (ExpInt (P4Int.Build_t _ i z None)) TypInteger dir.
+  Proof.
+    intros; soundtac.
+  Qed.
+
+  Lemma unsigned_int_sound : forall tag i z w dir,
+      Γ ⊢e
+        MkExpression
+        tag (ExpInt (P4Int.Build_t _ i z (Some (w,false)))) (TypBit w) dir.
+  Proof.
+    intros tag i z dir; soundtac.
+    (* TODO: need some result about [P4Arith.to_loptbool]. *)
+  Admitted.
+
+  Lemma signed_int_sound : forall tag i z w dir,
+      Γ ⊢e
+        MkExpression
+        tag (ExpInt (P4Int.Build_t _ i z (Some (w,true)))) (TypInt w) dir.
+  Proof.
+    intros tag i z dir; soundtac.
+    (* TODO: need some result about [P4Arith.to_loptbool]. *)
+  Admitted.
+
+  Lemma string_sound : forall tag s dir,
+      Γ ⊢e MkExpression tag (ExpString s) TypString dir.
+  Proof.
+    intros; soundtac.
+  Qed.
+
+  Lemma name_sound : forall tag x loc t dir,
+      typ_of_loc loc Γ = Some t ->
+      Γ ⊢e MkExpression tag (ExpName x loc) t dir.
+  Proof.
+    intros i x l t d Hgt; soundtac.
+    - destruct l as [lp | lp]; simpl in Hgt;
+        eapply envs_same_some_l in Hgt as [v Hv]; eauto.
+      exists v. constructor; simpl.
+      (** TODO:
+          1. Need type preservation to [eval_val_to_sval].
+          2. Perhaps [envs_same] needs to include [genv]. *)
+      admit.
+    - destruct l as [lp | lp]; simpl in Hgt;
+        simpl in *; eauto.
+  Abort.
+
+  Lemma array_access_sound : forall tag arry idx ts dir n,
+      typ_of_expr arry = TypArray (TypHeader ts) n ->
+      typ_of_expr idx  = TypBit n ->
+      Γ ⊢e arry ->
+      Γ ⊢e idx ->
+      Γ ⊢e MkExpression tag (ExpArrayAccess arry idx) (TypHeader ts) dir.
+  Proof.
+    intros i e1 e2 ts d n Ht1 Ht2 He1 He2;
+      autounfold with * in *.
+    intros rob ge p st Henvs Henvt.
+    pose proof He1 rob ge p st Henvs Henvt as [[v1 Hev1] He1']; clear He1.
+    pose proof He2 rob ge p st Henvs Henvt as [[v2 Hev2] He2']; clear He2.
+    split.
+    - pose proof He1' v1 Hev1 as Hv1.
+      pose proof He2' v2 Hev2 as Hv2.
+      rewrite Ht1 in Hv1; rewrite Ht2 in Hv2.
+      inversion Hv1; inversion Hv2; subst.
+      (* Need to know [N_of_value idx < n]. *) admit.
+    - intros v' Haa; inversion Haa; clear Haa; subst; simpl.
+      rename H4 into He2; rename H10 into He1;
+        rename H7 into Hsval; rename H9 into Haa;
+          rename H11 into Huninit.
+      pose proof He1' _ He1 as Hv1.
+      pose proof He2' _ He2 as Hv2.
+      rewrite Ht1 in Hv1; rewrite Ht2 in Hv2.
+      inversion Hv1; inversion Hv2; subst.
+      (* Need result about [Znth_def]. *)
+  Abort.
+
+  Lemma bigstring_access_sound : forall tag bits lo hi dir w,
+      (lo <= hi < w)%N ->
+      typ_of_expr bits = TypBit w ->
+      Γ ⊢e bits ->
+      Γ ⊢e MkExpression
+        tag (ExpBitStringAccess bits lo hi)
+        (TypBit (hi - lo + 1)%N) dir.
+  Proof.
+    intros i e lo hi d w Hlwh Ht He.
+    autounfold with * in *.
+    intros rob ge p st Henvs Henvt.
+    pose proof He rob ge p st Henvs Henvt as [[v Hev] He']; clear He.
+    split.
+    - apply He' in Hev as Hv; rewrite Ht in Hv;
+        inversion Hv; subst; rename v0 into bits.
+      exists (ValBaseBit (bitstring_slice bits (N.to_nat lo) (N.to_nat hi))).
+      eapply exec_expr_bitstring_access with (wn := length bits); eauto; lia.
+    - clear v Hev. intros v Hrn; inversion Hrn; subst; simpl.
+      rename H8 into He; rename H9 into Hsval; rename H12 into Hlhw.
+      (* Need result about [bitstring_slice]. *) admit.
+  Admitted.
+  
+  Lemma list_sound : forall tag es dir,
+      Forall (fun e => Γ ⊢e e) es ->
+      Γ ⊢e MkExpression tag (ExpList es)
+        (TypTuple (map typ_of_expr es)) dir.
+  Proof.
+    intros i es d Hes. autounfold with * in *.
+    intros rob ge p st Henvs Henvt.
+    rewrite Forall_forall in Hes.
+      specialize Hes with
+          (read_one_bit:=rob) (ge:=ge) (p:=p) (st:=st).
+      pose proof reduce_inner_impl _ _ _ _ Hes Henvs as Hes';
+        simpl in Hes'; clear Hes.
+      pose proof reduce_inner_impl _ _ _ _ Hes' Henvt as Hes;
+        simpl in Hes; clear Hes'.
+      rewrite split_impl_conj in Hes.
+      destruct Hes as [Hrnes Htyps]. split.
+    - clear Htyps; rewrite <- Forall_forall in Hrnes.
+      rewrite Forall_exists_factor in Hrnes.
+      destruct Hrnes as [vs Hvs]; eauto.
+    - clear Hrnes; intros v Hrn; simpl.
+      inversion Hrn; subst; clear Hrn.
+      rename H6 into Hesvs.
+      apply forall_Forall2 with (bs := vs) in Htyps;
+        eauto using Forall2_length.
+      apply Forall2_impl with
+          (R := run_expr ge rob p st)
+          (Q := fun e v => val_typ (ge_senum ge) v (typ_of_expr e)) in Htyps; auto.
+      rewrite Forall2_flip, Forall2_map_r in Htyps; auto.
+  Qed.
+  
+  Lemma record_sound : forall tag es dir,
+      Forall (fun e => Γ ⊢e e) (map snd es) ->
+      Γ ⊢e
+        MkExpression
+        tag (ExpRecord es)
+        (TypRecord (map (fun '(x,e) => (x,typ_of_expr e)) es)) dir.
+  Proof.
+    intros i es d Hes.
+    autounfold with * in *.
+    intros rob ge p st Henvs Henvt.
+    rewrite Forall_forall in Hes.
+    specialize Hes with
+        (read_one_bit:=rob) (ge:=ge) (p:=p) (st:=st).
+    pose proof reduce_inner_impl _ _ _ _ Hes Henvs as Hes';
+      simpl in Hes'; clear Hes.
+    pose proof reduce_inner_impl _ _ _ _ Hes' Henvt as Hes;
+      simpl in Hes; clear Hes'.
+    rewrite split_impl_conj in Hes.
+    destruct Hes as [Hrns Htyps]. split.
+    - clear Htyps. rewrite <- Forall_forall in Hrns.
+      rewrite Forall_exists_factor in Hrns.
+      destruct Hrns as [vs Hvs].
+      rewrite AList.Forall2_all_values
+        with (ks := map fst es) in Hvs.
+      + rewrite combine_map_fst_snd in Hvs; eauto.
+      + repeat rewrite map_length; reflexivity.
+      + rewrite map_length, <- map_length with (f := snd).
+        eauto using Forall2_length.
+    - clear Hrns; intros v Hrns.
+      inversion Hrns; subst.
+      rename H6 into Heskvs.
+      rewrite <- combine_map_fst_snd with (l := es)   in Heskvs.
+      rewrite <- combine_map_fst_snd with (l := kvs') in Heskvs.
+      apply AList.all_values_keys_eq in Heskvs as Hmf.
+      repeat rewrite combine_map_fst_snd in Hmf.
+      rewrite <- Hmf in Heskvs.
+      rewrite <- AList.Forall2_all_values in Heskvs.
+      + constructor; unfold AList.all_values;
+          rewrite Forall2_conj; split.
+        * rewrite Forall2_map_both, Forall2_eq,
+          map_fst_map, map_id; auto.
+        * rewrite Forall2_map_both.
+          rewrite map_snd_map.
+          assert (Hl : length es = length kvs').
+          { rewrite <- map_length with (f := fst) (l := es).
+            rewrite <- map_length with (f := fst) (l := kvs'), Hmf.
+            reflexivity. }
+          rewrite <- map_length with (f := snd) (l := es) in Hl.
+          rewrite <- map_length with (f := snd) (l := kvs') in Hl.
+          pose proof forall_Forall2 _ _ _ _ Htyps (map snd kvs') Hl as Hff2.
+          apply Forall2_impl with
+              (R := run_expr ge rob p st)
+              (Q := fun e v => val_typ (ge_senum ge) v (typ_of_expr e)) in Hff2; auto.
+          rewrite Forall2_flip,Forall2_map_r in Hff2; assumption.
+      + repeat rewrite map_length; reflexivity.
+      + rewrite Hmf; repeat rewrite map_length; reflexivity.
+  Qed.
+
+  (** Evidence for a type being a numeric of a given width. *)
+  Inductive numeric_width (w : N) : typ -> Prop :=
+  | numeric_width_bit : numeric_width w (TypBit w)
+  | numeric_width_int : numeric_width w (TypInt w).
+
+  Ltac inv_numeric_width :=
+    match goal with
+    | H: numeric_width _ _ |- _ => inversion H; subst
+    end.
+  
+  (** Evidence for a type being numeric. *)
+  Inductive numeric : typ -> Prop :=
+  | NumericFixed (w : N) τ :
+      numeric_width w τ -> numeric τ
+  | NumericArbitrary :
+      numeric TypInteger.
+
+  Ltac inv_numeric :=
+    match goal with
+    | H: numeric _ |- _ => inversion H; subst; try inv_numeric_width
+    end.
+
+  (** Evidence a unary operation is valid for a type. *)
+  Inductive unary_type : OpUni -> typ -> typ -> Prop :=
+  | UTBool :
+      unary_type Not TypBool TypBool
+  | UTBitNot w τ :
+      numeric_width w τ -> unary_type BitNot τ τ
+  | UTUMinus τ :
+      numeric τ -> unary_type UMinus τ τ.
+
+  Local Hint Constructors exec_val : core.
+  Local Hint Unfold read_detbit : core.
+  Local Hint Unfold sval_to_val : core.
+  Local Hint Unfold val_to_sval : core.
+  
+  Lemma val_to_sval_ex : forall v,
+      @val_to_sval tags_t v (ValueBaseMap Some v).
+  Proof.
+    autounfold with *; intro v.
+    induction v using (custom_ValueBase_ind bool); simpl; eauto.
+    - constructor.
+      rewrite <- Forall2_map_r, Forall2_Forall, Forall_forall.
+      reflexivity.
+    - constructor.
+      rewrite <- Forall2_map_r, Forall2_Forall, Forall_forall.
+      reflexivity.
+    - constructor.
+      rewrite <- Forall2_map_r, Forall2_Forall, Forall_forall.
+      reflexivity.
+    - constructor.
+      rewrite <- Forall2_map_r, Forall2_Forall.
+      assumption.
+    - constructor. unfold AList.all_values.
+      rewrite <- Forall2_map_r, Forall2_Forall.
+      rewrite Forall_snd in H.
+      apply Forall_and; rewrite Forall_forall in *;
+        intros [? ?]; firstorder.
+    - constructor. unfold AList.all_values.
+      rewrite <- Forall2_map_r, Forall2_Forall.
+      rewrite Forall_snd in H.
+      apply Forall_and; rewrite Forall_forall in *;
+        intros [? ?]; firstorder.
+    - constructor; auto. unfold AList.all_values.
+      rewrite <- Forall2_map_r, Forall2_Forall.
+      rewrite Forall_snd in H.
+      apply Forall_and; rewrite Forall_forall in *;
+        intros [? ?]; firstorder.
+    - constructor. unfold AList.all_values.
+      rewrite <- Forall2_map_r, Forall2_Forall.
+      rewrite Forall_snd in H.
+      apply Forall_and; rewrite Forall_forall in *;
+        intros [? ?]; firstorder.
+    - constructor.
+      rewrite <- Forall2_map_r, Forall2_Forall.
+      assumption.
+  Qed.
+
+  Local Hint Resolve val_to_sval_ex : core.
+
+  Lemma unary_type_eq : forall o t t', unary_type o t t' -> t = t'.
+  Proof.
+    intros ? ? ? H; inversion H; subst; auto.
+  Qed.
+  
+  Lemma unary_op_sound : forall tag o e t dir,
+      unary_type o (typ_of_expr e) t ->
+      Γ ⊢e e ->
+      Γ ⊢e MkExpression tag (ExpUnaryOp o e) t dir.
+  Proof.
+    intros i o e t d Hut He.
+    autounfold with * in *;
+      intros rob ge p st Henvs Henvt.
+    specialize He with rob ge p st.
+    pose proof He Henvs Henvt as [[v Hev] Hvt]; clear He; split.
+    - apply Hvt in Hev as Hv; clear Hvt.
+      assert (exists v', sval_to_val rob v v').
+      { admit. }
+      (* Need predicate that [rob v v'] holds in [expr_types]... *)
+      destruct H as [v' Hv'].
+      destruct (Ops.Ops.eval_unary_op o v') as [v'' |] eqn:Heqop; eauto.
+      inversion Hut; subst; try inv_numeric; try inv_numeric_width;
+        match goal with
+        | H: _ = typ_of_expr ?e,
+             Hv: val_typ _ ?v (typ_of_expr ?e),
+                 Hv': sval_to_val _ ?v _
+          |- _ => rewrite <- H in *; inversion Hv; inversion Hv'; subst
+        end; simpl in *; try discriminate.
+    - clear v Hev; intros v Hev.
+      inversion Hev; subst; simpl in *.
+      pose proof Hvt _ H7 as Hargsv.
+      (* Need to know:
+         - [forall o t t', unary_type o t t' -> t = t']
+         - [forall f g t v v', exec_val f v v' -> val_typ g v t -> val_typ g v' t]
+         - [forall o v v' g t, eval_unary_op o v = Some v' -> val_typ g v t -> val_typ g v' t].
+         Requires a parameterized [val_typ]. *)
+  Abort.
+End Soundness.
